MPPA - Ocast32signed

mppa_k1c/Asmexpand.ml
@@ -551,11 +551,12 @@ let expand_instruction instr =
 *)| Pcvtl2w(rd, rs) ->
       assert Archi.ptr64;
       emit (Paddiw(rd, rs, Int.zero))  (* 32-bit sign extension *)
-(*| Pcvtw2l(r) ->
+  | Pcvtw2l(r) ->
       assert Archi.ptr64
       (* no-operation because the 32-bit integer was kept sign extended already *)
+      (* FIXME - is it really the case on the MPPA ? *)
 
-  | Pjal_r(r, sg) ->
+(*| Pjal_r(r, sg) ->
       fixup_call sg; emit instr
   | Pjal_s(symb, sg) ->
       fixup_call sg; emit instr
